state/Examples.HO.fst
@@ -15,29 +15,29 @@ open SpecTree
 
 #set-options "--print_universes"
 
-type f_eqx (pspec:poly_iface_pspec) = x:ref int -> ST (resexn unit) (requires (fun h0 -> (Mktuple3?._1 pspec) h0 /\ satisfy x (prref_c))) (ensures (fun h0 r h1 -> (Mktuple3?._1 pspec) h1 /\ (Mktuple3?._3 pspec) h0 h1 /\ (Inr? r \/ sel h0 x == sel h1 x)))
+type f_eqx (a3p:threep) = x:ref int -> ST (resexn unit) (requires (fun h0 -> (Mktuple3?._1 a3p) h0 /\ satisfy x (prref_c))) (ensures (fun h0 r h1 -> (Mktuple3?._1 a3p) h1 /\ (Mktuple3?._3 a3p) h0 h1 /\ (Inr? r \/ sel h0 x == sel h1 x)))
 
-let f_pspec pspec : pck_spec pspec =
- (SpecErr false (ref int) (exportable_refinement pspec
+let f_a3p a3p : pck_spec a3p =
+ (SpecErr false (ref int) (exportable_refinement a3p
                   (ref int)
                   Leaf
                   (fun _ -> l_True))
                 .c_styp
-              (fun x h0 -> (Mktuple3?._1 pspec) h0 /\ satisfy x (prref_c))
+              (fun x h0 -> (Mktuple3?._1 a3p) h0 /\ satisfy x (prref_c))
               unit
-              (safe_importable_is_importable pspec unit Leaf).c_styp
-              (fun x h0 r h1 -> (Mktuple3?._1 pspec) h1 /\ (Mktuple3?._3 pspec) h0 h1 /\ (Inr? r \/ sel h0 x == sel h1 x)))
+              (safe_importable_is_importable a3p unit Leaf).c_styp
+              (fun x h0 r h1 -> (Mktuple3?._1 a3p) h1 /\ (Mktuple3?._3 a3p) h0 h1 /\ (Inr? r \/ sel h0 x == sel h1 x)))
 
-let f_spec : pck_spec concrete_spec = f_pspec concrete_spec
+let f_spec : pck_spec concrete_spec = f_a3p concrete_spec
 
-let f_eqx_is_safe_importable pspec : safe_importable_to pspec (f_eqx pspec) (Node (f_pspec pspec) Leaf Leaf) =
+let f_eqx_is_safe_importable a3p : safe_importable_to a3p (f_eqx a3p) (Node (f_a3p a3p) Leaf Leaf) =
   solve
 (**
-  safe_importable_arrow pspec
+  safe_importable_arrow a3p
     (ref int) unit
     Leaf Leaf
-    (fun x h0 -> (Mktuple3?._1 pspec) h0 /\ satisfy x (prref_c))
-    (fun x h0 r h1 -> (Mktuple3?._1 pspec) h1 /\ (Mktuple3?._3 pspec) h0 h1 /\ (Inr? r \/ sel h0 x == sel h1 x))**)
+    (fun x h0 -> (Mktuple3?._1 a3p) h0 /\ satisfy x (prref_c))
+    (fun x h0 r h1 -> (Mktuple3?._1 a3p) h1 /\ (Mktuple3?._3 a3p) h0 h1 /\ (Inr? r \/ sel h0 x == sel h1 x))**)
 
 let f_hoc : hoc concrete_spec f_spec =
 EnforcePost
@@ -59,7 +59,7 @@ let f_tree : hoc_tree (Node f_spec Leaf Leaf) =
   Node f_pkhoc Leaf Leaf
 
 let sit : src_interface1 = {
-  specs = (fun preds -> Node (f_pspec preds) Leaf Leaf);
+  specs = (fun preds -> Node (f_a3p preds) Leaf Leaf);
   hocs = f_tree;
   ct = f_eqx;
   c_ct = f_eqx_is_safe_importable;
