state/HigherOrderContracts.fst
@@ -9,46 +9,46 @@ open Witnessable
 open PolyIface
 open SpecTree
 
-instance poly_iface_err pspec : poly_iface pspec err = {
+instance poly_iface_err a3p : poly_iface a3p err = {
   wt = witnessable_err
 }
 
-class exportable_from pspec (styp: Type u#a) (st:spec_tree pspec) = {
+class exportable_from a3p (styp: Type u#a) (st:spec_tree a3p) = {
   [@@@no_method] c_styp : witnessable styp;
   [@@@no_method] ityp : Type u#b;
-  [@@@no_method] c_ityp : poly_iface pspec ityp;
+  [@@@no_method] c_ityp : poly_iface a3p ityp;
   [@@@no_method] export : hoc_tree st -> styp -> ityp;
   [@@@no_method] lemma_export_preserves_prref :
     x:styp -> prref:mref_pred -> hocs:hoc_tree st -> Lemma (requires (c_styp.satisfy x prref)) (ensures (c_ityp.wt.satisfy (export hocs x) (prref)))
 }
 
-class safe_importable_to pspec (styp: Type u#a) (st:spec_tree pspec) = {
+class safe_importable_to a3p (styp: Type u#a) (st:spec_tree a3p) = {
   [@@@no_method] c_styp : witnessable styp;
   [@@@no_method] ityp : Type u#b;
-  [@@@no_method] c_ityp : poly_iface pspec ityp;
+  [@@@no_method] c_ityp : poly_iface a3p ityp;
   [@@@no_method] safe_import : ityp -> hoc_tree st -> styp;
   [@@@no_method] lemma_safe_import_preserves_prref :
     x:ityp -> prref:mref_pred -> hocs:hoc_tree st -> Lemma (requires (c_ityp.wt.satisfy x (prref))) (ensures (c_styp.satisfy (safe_import x hocs) (prref)))
 }
 
-class importable_to pspec (styp: Type u#a) (st:spec_tree pspec) = {
+class importable_to a3p (styp: Type u#a) (st:spec_tree a3p) = {
   [@@@no_method] c_styp : witnessable styp;
   [@@@no_method] ityp : Type u#b;
-  [@@@no_method] c_ityp : poly_iface pspec ityp;
+  [@@@no_method] c_ityp : poly_iface a3p ityp;
   [@@@no_method] import : ityp -> hoc_tree st -> resexn styp;
   [@@@no_method] lemma_import_preserves_prref :
     x:ityp -> prref:mref_pred -> hocs:hoc_tree st -> Lemma (requires (c_ityp.wt.satisfy x prref)) (ensures ((witnessable_sum styp err).satisfy (import x hocs) prref))
 }
 
 (** Exportable instances **)
-instance poly_iface_is_exportable t pspec {| c1:poly_iface pspec t |} : exportable_from pspec t Leaf = {
+instance poly_iface_is_exportable t a3p {| c1:poly_iface a3p t |} : exportable_from a3p t Leaf = {
   c_styp = c1.wt;
   ityp = t;
   c_ityp = solve;
   export = (fun Leaf x -> x);
   lemma_export_preserves_prref = (fun _ _ _ -> ()) }
 
-instance exportable_unit pspec : exportable_from pspec unit Leaf = {
+instance exportable_unit a3p : exportable_from a3p unit Leaf = {
   c_styp = witnessable_unit;
   ityp = unit;
   c_ityp = poly_iface_unit _;
@@ -56,7 +56,7 @@ instance exportable_unit pspec : exportable_from pspec unit Leaf = {
   lemma_export_preserves_prref = (fun _ _ _ -> ())
 }
 
-instance exportable_err pspec : exportable_from pspec err Leaf = {
+instance exportable_err a3p : exportable_from a3p err Leaf = {
   c_styp = witnessable_err;
   ityp = err;
   c_ityp = poly_iface_err _;
@@ -64,7 +64,7 @@ instance exportable_err pspec : exportable_from pspec err Leaf = {
   lemma_export_preserves_prref = (fun _ _ _ -> ())
 }
 
-instance exportable_int pspec : exportable_from pspec int Leaf = {
+instance exportable_int a3p : exportable_from a3p int Leaf = {
   c_styp = witnessable_int;
   ityp = int;
   c_ityp = poly_iface_int _;
@@ -72,7 +72,7 @@ instance exportable_int pspec : exportable_from pspec int Leaf = {
   lemma_export_preserves_prref = (fun _ _ _ -> ())
 }
 
-instance exportable_option pspec t specs {| c:exportable_from pspec t specs |} : exportable_from pspec (option t) specs = {
+instance exportable_option a3p t specs {| c:exportable_from a3p t specs |} : exportable_from a3p (option t) specs = {
   c_styp = witnessable_option t #c.c_styp;
   ityp = option c.ityp;
   c_ityp = poly_iface_option _ c.ityp #c.c_ityp;
@@ -80,7 +80,7 @@ instance exportable_option pspec t specs {| c:exportable_from pspec t specs |} :
   lemma_export_preserves_prref = (fun x p hocs -> match x with | Some x -> c.lemma_export_preserves_prref x p hocs | None -> ())
 }
 
-instance exportable_sum pspec t1 t2 s1 s2 {| c1:exportable_from pspec t1 s1 |} {| c2:exportable_from pspec t2 s2 |} : exportable_from pspec (either t1 t2) (EmptyNode s1 s2) = {
+instance exportable_sum a3p t1 t2 s1 s2 {| c1:exportable_from a3p t1 s1 |} {| c2:exportable_from a3p t2 s2 |} : exportable_from a3p (either t1 t2) (EmptyNode s1 s2) = {
   c_styp = witnessable_sum t1 t2 #c1.c_styp #c2.c_styp;
   ityp = either c1.ityp c2.ityp;
   c_ityp = poly_iface_sum _ _ _ #c1.c_ityp #c2.c_ityp;
@@ -89,10 +89,10 @@ instance exportable_sum pspec t1 t2 s1 s2 {| c1:exportable_from pspec t1 s1 |} {
     match x with | Inl x -> c1.lemma_export_preserves_prref x p (left hocs)| Inr x -> c2.lemma_export_preserves_prref x p (right hocs))
 }
 
-instance exportable_resexn pspec t spec {| c:exportable_from pspec t spec |} : exportable_from pspec (resexn t) (EmptyNode spec Leaf) =
-  exportable_sum pspec t err spec Leaf #c #(exportable_err pspec)
+instance exportable_resexn a3p t spec {| c:exportable_from a3p t spec |} : exportable_from a3p (resexn t) (EmptyNode spec Leaf) =
+  exportable_sum a3p t err spec Leaf #c #(exportable_err a3p)
 
-instance exportable_pair pspec t1 t2 s1 s2 {| c1:exportable_from pspec t1 s1 |} {| c2:exportable_from pspec t2 s2 |} : exportable_from pspec (t1 * t2) (EmptyNode s1 s2) = {
+instance exportable_pair a3p t1 t2 s1 s2 {| c1:exportable_from a3p t1 s1 |} {| c2:exportable_from a3p t2 s2 |} : exportable_from a3p (t1 * t2) (EmptyNode s1 s2) = {
   c_styp = witnessable_pair t1 t2 #c1.c_styp #c2.c_styp;
   ityp = c1.ityp * c2.ityp;
   c_ityp = poly_iface_pair _ _ _ #c1.c_ityp #c2.c_ityp;
@@ -100,7 +100,7 @@ instance exportable_pair pspec t1 t2 s1 s2 {| c1:exportable_from pspec t1 s1 |} 
   lemma_export_preserves_prref = (fun (x1, x2) p hocs -> c1.lemma_export_preserves_prref x1 p (left hocs); c2.lemma_export_preserves_prref x2 p (right hocs))
 }
 
-instance exportable_ref pspec t {| c:tc_shareable_type t |} : exportable_from pspec (ref t) Leaf = {
+instance exportable_ref a3p t {| c:tc_shareable_type t |} : exportable_from a3p (ref t) Leaf = {
   c_styp = witnessable_mref t _ #solve;
   ityp = ref t;
   c_ityp = poly_iface_ref _ t #c;
@@ -108,8 +108,8 @@ instance exportable_ref pspec t {| c:tc_shareable_type t |} : exportable_from ps
   lemma_export_preserves_prref = (fun _ _ _ -> ());
 }
 
-instance exportable_llist pspec t {| c:tc_shareable_type t |} :
-  exportable_from pspec (linkedList t) Leaf = {
+instance exportable_llist a3p t {| c:tc_shareable_type t |} :
+  exportable_from a3p (linkedList t) Leaf = {
   c_styp = solve ;
   ityp = linkedList t ;
   c_ityp = solve ;
@@ -117,7 +117,7 @@ instance exportable_llist pspec t {| c:tc_shareable_type t |} :
   lemma_export_preserves_prref = (fun _ _ _ -> ())
 }
 
-instance exportable_refinement pspec t spec {| c:exportable_from pspec t spec |} (p:t->Type0) : exportable_from pspec (x:t{p x}) spec = {
+instance exportable_refinement a3p t spec {| c:exportable_from a3p t spec |} (p:t->Type0) : exportable_from a3p (x:t{p x}) spec = {
   c_styp = witnessable_refinement t #c.c_styp p;
   ityp = c.ityp;
   c_ityp = c.c_ityp;
@@ -126,36 +126,36 @@ instance exportable_refinement pspec t spec {| c:exportable_from pspec t spec |}
 }
 
 instance exportable_arrow
-  pspec
+  a3p
   (t1:Type) (t2:Type)
   s1 s2
-  {| c1:importable_to pspec t1 s1 |}
-  {| c2:exportable_from pspec t2 s2 |}
+  {| c1:importable_to a3p t1 s1 |}
+  {| c2:exportable_from a3p t2 s2 |}
   (pre:(t1 -> st_pre))
   (post:(x:t1 -> h0:heap -> st_post' (resexn t2) (pre x h0)))
- // (_:squash (forall x h0 r h1. post x h0 r h1 ==> post_poly_iface_arrow pspec #(resexn t2) #(witnessable_sum t2 err #c2.c_styp) h0 r h1))
- // (check:select_check pspec t1 unit (pre_poly_iface_arrow pspec #_ #c1.c_styp)
+ // (_:squash (forall x h0 r h1. post x h0 r h1 ==> post_poly_iface_arrow a3p #(resexn t2) #(witnessable_sum t2 err #c2.c_styp) h0 r h1))
+ // (check:select_check a3p t1 unit (pre_poly_iface_arrow a3p #_ #c1.c_styp)
  //   (fun x _ _ h1 -> pre x h1))
                 (** ^ the fact that the check has a pre-condition means that the check does not have to enforce it
                       e.g., the invariant on the heap **)
-  : exportable_from pspec (x:t1 -> ST (resexn t2) (pre x) (post x))
+  : exportable_from a3p (x:t1 -> ST (resexn t2) (pre x) (post x))
     (Node (SpecErr true t1 c1.c_styp pre t2 c2.c_styp post) s1 s2) = {
   c_styp = witnessable_arrow t1 (resexn t2) pre post;
-  ityp = mk_poly_iface_arrow pspec c1.ityp #c1.c_ityp.wt (resexn c2.ityp) #(witnessable_resexn #c2.ityp #c2.c_ityp.wt);
-  c_ityp = poly_iface_arrow pspec c1.ityp (resexn c2.ityp) #c1.c_ityp #(poly_iface_sum pspec c2.ityp err #c2.c_ityp) ;
+  ityp = mk_poly_iface_arrow a3p c1.ityp #c1.c_ityp.wt (resexn c2.ityp) #(witnessable_resexn #c2.ityp #c2.c_ityp.wt);
+  c_ityp = poly_iface_arrow a3p c1.ityp (resexn c2.ityp) #c1.c_ityp #(poly_iface_sum a3p c2.ityp err #c2.c_ityp) ;
   export = (fun (hocs:hoc_tree _) (f:(x:t1 -> ST (resexn t2) (pre x) (post x))) (x:c1.ityp) ->
     let Node (| _, myhoc |) lhs rhs : hoc_tree _ = hocs in
     let EnforcePre check c_post = myhoc in
     match c1.import x lhs with
     | Inl x' -> begin
-      c1.lemma_import_preserves_prref x (Mktuple3?._2 pspec) lhs;
+      c1.lemma_import_preserves_prref x (Mktuple3?._2 a3p) lhs;
       let (| _, cb_check |) = check x' in
       match cb_check () with
       | Inl _ -> begin
         let res : resexn t2 = f x' in
         c_post x' res;
-        (exportable_resexn pspec t2 s2).lemma_export_preserves_prref res (Mktuple3?._2 pspec) (EmptyNode rhs Leaf);
-        (exportable_resexn pspec t2 s2).export (EmptyNode rhs Leaf) res
+        (exportable_resexn a3p t2 s2).lemma_export_preserves_prref res (Mktuple3?._2 a3p) (EmptyNode rhs Leaf);
+        (exportable_resexn a3p t2 s2).export (EmptyNode rhs Leaf) res
       end
       | Inr err -> Inr err
     end
@@ -165,7 +165,7 @@ instance exportable_arrow
 }
 
 (** Importable instances **)
-instance poly_iface_is_safely_importable pspec t {| c1:poly_iface pspec t |} : safe_importable_to pspec t Leaf = {
+instance poly_iface_is_safely_importable a3p t {| c1:poly_iface a3p t |} : safe_importable_to a3p t Leaf = {
   c_styp = c1.wt;
   ityp = t;
   c_ityp = solve;
@@ -173,7 +173,7 @@ instance poly_iface_is_safely_importable pspec t {| c1:poly_iface pspec t |} : s
   lemma_safe_import_preserves_prref = (fun _ _ _ -> ())
 }
 
-instance safe_importable_is_importable pspec t spec {| c1:safe_importable_to pspec t spec |} : importable_to pspec t spec = {
+instance safe_importable_is_importable a3p t spec {| c1:safe_importable_to a3p t spec |} : importable_to a3p t spec = {
   c_styp = c1.c_styp;
   ityp = c1.ityp;
   c_ityp = c1.c_ityp;
@@ -181,7 +181,7 @@ instance safe_importable_is_importable pspec t spec {| c1:safe_importable_to psp
   lemma_import_preserves_prref = (fun x -> c1.lemma_safe_import_preserves_prref x);
 }
 
-instance safe_importable_unit pspec : safe_importable_to pspec unit Leaf = {
+instance safe_importable_unit a3p : safe_importable_to a3p unit Leaf = {
   c_styp = witnessable_unit;
   ityp = unit;
   c_ityp = poly_iface_unit _;
@@ -189,7 +189,7 @@ instance safe_importable_unit pspec : safe_importable_to pspec unit Leaf = {
   lemma_safe_import_preserves_prref = (fun _ _ _ -> ())
 }
 
-instance safe_importable_err pspec : safe_importable_to pspec err Leaf = {
+instance safe_importable_err a3p : safe_importable_to a3p err Leaf = {
   c_styp = witnessable_err;
   ityp = err;
   c_ityp = poly_iface_err _;
@@ -197,7 +197,7 @@ instance safe_importable_err pspec : safe_importable_to pspec err Leaf = {
   lemma_safe_import_preserves_prref = (fun _ _ _ -> ())
 }
 
-instance importable_option pspec t spec {| c:importable_to pspec t spec |} : importable_to pspec (option t) spec = {
+instance importable_option a3p t spec {| c:importable_to a3p t spec |} : importable_to a3p (option t) spec = {
   c_styp = witnessable_option t #c.c_styp;
   ityp = option c.ityp;
   c_ityp = poly_iface_option _ c.ityp #c.c_ityp;
@@ -215,7 +215,7 @@ instance importable_option pspec t spec {| c:importable_to pspec t spec |} : imp
     | None -> ())
 }
 
-instance importable_sum pspec t1 t2 s1 s2 {| c1:importable_to pspec t1 s1 |} {| c2:importable_to pspec t2 s2 |} : importable_to pspec (either t1 t2) (EmptyNode s1 s2) = {
+instance importable_sum a3p t1 t2 s1 s2 {| c1:importable_to a3p t1 s1 |} {| c2:importable_to a3p t2 s2 |} : importable_to a3p (either t1 t2) (EmptyNode s1 s2) = {
   c_styp = witnessable_sum t1 t2 #c1.c_styp #c2.c_styp;
   ityp = either c1.ityp c2.ityp;
   c_ityp = poly_iface_sum _ _ _ #c1.c_ityp #c2.c_ityp;
@@ -237,7 +237,7 @@ instance importable_sum pspec t1 t2 s1 s2 {| c1:importable_to pspec t1 s1 |} {| 
     | Inr x -> c2.lemma_import_preserves_prref x p (right hocs))
 }
 
-instance importable_pair pspec t1 t2 s1 s2 {| c1:importable_to pspec t1 s1 |} {| c2:importable_to pspec t2 s2 |} : importable_to pspec (t1 * t2) (EmptyNode s1 s2) = {
+instance importable_pair a3p t1 t2 s1 s2 {| c1:importable_to a3p t1 s1 |} {| c2:importable_to a3p t2 s2 |} : importable_to a3p (t1 * t2) (EmptyNode s1 s2) = {
   c_styp = witnessable_pair t1 t2 #c1.c_styp #c2.c_styp;
   ityp = c1.ityp * c2.ityp;
   c_ityp = poly_iface_pair _ _ _ #c1.c_ityp #c2.c_ityp;
@@ -254,7 +254,7 @@ instance importable_pair pspec t1 t2 s1 s2 {| c1:importable_to pspec t1 s1 |} {|
     c2.lemma_import_preserves_prref (snd x) p (right hocs))
 }
 
-instance safe_importable_ref pspec t {| c:tc_shareable_type t |} : safe_importable_to pspec (ref t) Leaf = {
+instance safe_importable_ref a3p t {| c:tc_shareable_type t |} : safe_importable_to a3p (ref t) Leaf = {
   c_styp = witnessable_mref t _ #solve;
   ityp = ref t;
   c_ityp = poly_iface_ref _ t;
@@ -262,7 +262,7 @@ instance safe_importable_ref pspec t {| c:tc_shareable_type t |} : safe_importab
   lemma_safe_import_preserves_prref = (fun _ _ _ -> ())
 }
 
-instance import_refinement pspec t spec {| c:importable_to pspec t spec |} (p:t->Type0) (check:(x:t -> r:bool{r ==> p x})): importable_to pspec (x:t{p x}) spec = {
+instance import_refinement a3p t spec {| c:importable_to a3p t spec |} (p:t->Type0) (check:(x:t -> r:bool{r ==> p x})): importable_to a3p (x:t{p x}) spec = {
   c_styp = witnessable_refinement t #c.c_styp p;
   ityp = c.ityp;
   c_ityp = c.c_ityp;
@@ -273,7 +273,7 @@ instance import_refinement pspec t spec {| c:importable_to pspec t spec |} (p:t-
   lemma_import_preserves_prref = (fun x -> c.lemma_import_preserves_prref x);
 }
 
-instance safe_importable_resexn pspec t s {| c:importable_to pspec t s |} : safe_importable_to pspec (resexn t) (EmptyNode s Leaf)= {
+instance safe_importable_resexn a3p t s {| c:importable_to a3p t s |} : safe_importable_to a3p (resexn t) (EmptyNode s Leaf)= {
   c_styp = witnessable_sum t err #c.c_styp;
   ityp = resexn c.ityp;
   c_ityp = poly_iface_sum _ c.ityp err #c.c_ityp;
@@ -293,30 +293,30 @@ instance safe_importable_resexn pspec t s {| c:importable_to pspec t s |} : safe
 }
 
 instance safe_importable_arrow
-  pspec
+  a3p
   (t1:Type) (t2:Type)
   s1 s2
-  {| c1:exportable_from pspec t1 s1 |}
-  {| c2:importable_to pspec t2 s2 |}
+  {| c1:exportable_from a3p t1 s1 |}
+  {| c2:importable_to a3p t2 s2 |}
   (pre:(t1 -> st_pre))
   (post:(x:t1 -> h0:heap -> st_post' (resexn t2) (pre x h0)))
- // (_:squash (forall (x:t1) h0. pre x h0 ==> pre_poly_iface_arrow pspec #_ #c1.c_styp x h0))
-//  (_:squash (forall (x:t1) h0 e h1. pre x h0 /\ post_poly_iface_arrow pspec #_ #(witnessable_sum t2 err #c2.c_styp) h0 (Inr e) h1 ==> post x h0 (Inr e) h1))
-//  (capture_check:select_check pspec t1 (resexn t2) #(witnessable_sum _ err #c2.c_styp) pre post)
-  : safe_importable_to pspec (x:t1 -> ST (resexn t2) (pre x) (post x)) (Node (SpecErr false t1 c1.c_styp pre t2 c2.c_styp post) s1 s2) = {
+ // (_:squash (forall (x:t1) h0. pre x h0 ==> pre_poly_iface_arrow a3p #_ #c1.c_styp x h0))
+//  (_:squash (forall (x:t1) h0 e h1. pre x h0 /\ post_poly_iface_arrow a3p #_ #(witnessable_sum t2 err #c2.c_styp) h0 (Inr e) h1 ==> post x h0 (Inr e) h1))
+//  (capture_check:select_check a3p t1 (resexn t2) #(witnessable_sum _ err #c2.c_styp) pre post)
+  : safe_importable_to a3p (x:t1 -> ST (resexn t2) (pre x) (post x)) (Node (SpecErr false t1 c1.c_styp pre t2 c2.c_styp post) s1 s2) = {
   c_styp = witnessable_arrow t1 (resexn t2) pre post;
-  ityp = mk_poly_iface_arrow pspec c1.ityp #c1.c_ityp.wt (resexn c2.ityp) #(witnessable_resexn #c2.ityp #c2.c_ityp.wt);
+  ityp = mk_poly_iface_arrow a3p c1.ityp #c1.c_ityp.wt (resexn c2.ityp) #(witnessable_resexn #c2.ityp #c2.c_ityp.wt);
   c_ityp = poly_iface_arrow _ c1.ityp (resexn c2.ityp) #_ #(poly_iface_sum _ c2.ityp err #c2.c_ityp);
-  safe_import = (fun (f:mk_poly_iface_arrow pspec c1.ityp #c1.c_ityp.wt (resexn c2.ityp) #(witnessable_sum c2.ityp err #c2.c_ityp.wt)) (hocs:hoc_tree _) (x:t1) ->
+  safe_import = (fun (f:mk_poly_iface_arrow a3p c1.ityp #c1.c_ityp.wt (resexn c2.ityp) #(witnessable_sum c2.ityp err #c2.c_ityp.wt)) (hocs:hoc_tree _) (x:t1) ->
     let Node (| _, myhoc |) lhs rhs : hoc_tree _ = hocs in
     let EnforcePost c_pre c_post check = myhoc in
     c_pre x;
-    c1.lemma_export_preserves_prref x (Mktuple3?._2 pspec) lhs;
+    c1.lemma_export_preserves_prref x (Mktuple3?._2 a3p) lhs;
     let (| _, cb_check |) = check x in
     let x' = c1.export lhs x in
     let res : resexn c2.ityp = f x' in
-    let fres = (safe_importable_resexn pspec t2 s2).safe_import res (EmptyNode rhs Leaf) in
-    (safe_importable_resexn pspec t2 s2).lemma_safe_import_preserves_prref res (Mktuple3?._2 pspec) (EmptyNode rhs Leaf);
+    let fres = (safe_importable_resexn a3p t2 s2).safe_import res (EmptyNode rhs Leaf) in
+    (safe_importable_resexn a3p t2 s2).lemma_safe_import_preserves_prref res (Mktuple3?._2 a3p) (EmptyNode rhs Leaf);
     match cb_check fres with
     | Inl _ -> fres
     | Inr err -> (c_post x err; (Inr err))
@@ -325,29 +325,29 @@ instance safe_importable_arrow
 }
 
 instance safe_importable_arrow_safe
-  pspec
+  a3p
   (t1:Type) (t2:Type)
   s1 s2
-  {| c1:exportable_from pspec t1 s1 |}
-  {| c2:safe_importable_to pspec t2 s2 |}
+  {| c1:exportable_from a3p t1 s1 |}
+  {| c2:safe_importable_to a3p t2 s2 |}
   (pre:(t1 -> st_pre))
   (post:(x:t1 -> h0:heap -> st_post' t2 (pre x h0)))
- // (_:squash (forall (x:t1) h0. pre x h0 ==> pre_poly_iface_arrow pspec #_ #c1.c_styp x h0))
-//  (_:squash (forall (x:t1) h0 r h1. pre x h0 /\ post_poly_iface_arrow pspec #_ #c2.c_styp h0 r h1 ==> post x h0 r h1))
-  : safe_importable_to pspec (x:t1 -> ST t2 (pre x) (post x)) (Node (Spec false t1 c1.c_styp pre t2 c2.c_styp post) s1 s2) = {
+ // (_:squash (forall (x:t1) h0. pre x h0 ==> pre_poly_iface_arrow a3p #_ #c1.c_styp x h0))
+//  (_:squash (forall (x:t1) h0 r h1. pre x h0 /\ post_poly_iface_arrow a3p #_ #c2.c_styp h0 r h1 ==> post x h0 r h1))
+  : safe_importable_to a3p (x:t1 -> ST t2 (pre x) (post x)) (Node (Spec false t1 c1.c_styp pre t2 c2.c_styp post) s1 s2) = {
   c_styp = witnessable_arrow t1 t2 pre post;
-  ityp = mk_poly_iface_arrow pspec c1.ityp #c1.c_ityp.wt c2.ityp #c2.c_ityp.wt;
+  ityp = mk_poly_iface_arrow a3p c1.ityp #c1.c_ityp.wt c2.ityp #c2.c_ityp.wt;
   c_ityp = poly_iface_arrow _ c1.ityp c2.ityp #_ #c2.c_ityp;
-  safe_import = (fun (f:mk_poly_iface_arrow pspec c1.ityp #c1.c_ityp.wt c2.ityp #c2.c_ityp.wt) hocs (x:t1) ->
+  safe_import = (fun (f:mk_poly_iface_arrow a3p c1.ityp #c1.c_ityp.wt c2.ityp #c2.c_ityp.wt) hocs (x:t1) ->
     let Node (| _, myhoc |) lhs rhs : hoc_tree _ = hocs in
     let TrivialPost c_pre c_post = myhoc in
     c_pre x;
-    c1.lemma_export_preserves_prref x (Mktuple3?._2 pspec) lhs;
+    c1.lemma_export_preserves_prref x (Mktuple3?._2 a3p) lhs;
     let x' = c1.export lhs x in
     let res : c2.ityp = f x' in
     let fres = c2.safe_import res rhs in
     c_post x fres;
-    c2.lemma_safe_import_preserves_prref res (Mktuple3?._2 pspec) rhs;
+    c2.lemma_safe_import_preserves_prref res (Mktuple3?._2 a3p) rhs;
     fres
   );
   lemma_safe_import_preserves_prref = (fun _ _ _ -> ())
